Communication_Topology_Soundness.thy
@@ -6,6 +6,20 @@ theory Communication_Topology_Soundness
     Communication_Topology_Analysis
 begin
 
+theorem topology_pair_sound : "
+  \<lbrakk>
+    (x, t) \<Turnstile>\<^sub>t e; 
+    [[] \<mapsto> <<e, empty, []>>] \<rightarrow>* \<E>'
+  \<rbrakk> \<Longrightarrow>
+  \<langle>\<langle>\<E>' ; Ch \<pi> x\<rangle>\<rangle> \<preceq> t
+"
+sorry
+
+lemma topology_sound': "
+  (x, \<A> x) \<Turnstile>\<^sub>t e \<Longrightarrow> [[] \<mapsto> <<e,Map.empty,[]>>] \<rightarrow>* \<E>' \<Longrightarrow> (\<langle>\<langle>\<E>'\<rangle>\<rangle>) x \<preceq> \<A> x
+"
+sorry
+
 theorem topology_sound : "
   \<lbrakk>
     \<A> \<bind> e; 
@@ -13,7 +27,14 @@ theorem topology_sound : "
   \<rbrakk> \<Longrightarrow>
   \<langle>\<langle>\<E>'\<rangle>\<rangle> \<sqsubseteq>\<^sub>t \<A>
 "
- sorry
+ apply (unfold communication_topology_def)
+ apply (unfold topo_env_precision_def)
+ apply (intro allI, drule spec)
+ apply (erule topology_sound', auto)
+done
+ 
+
+
 
 
 end
